Parameterize get_machine_event

src/model/PFConfiguration.v
@@ -3,6 +3,7 @@ From Paco Require Import paco.
 
 From PromisingLib Require Import Axioms.
 From PromisingLib Require Import Basic.
+From PromisingLib Require Import Loc.
 From PromisingLib Require Import DataStructure.
 From PromisingLib Require Import DenseOrder.
 From PromisingLib Require Import Language.
@@ -25,58 +26,29 @@ Set Implicit Arguments.
 
 
 Module PFConfiguration.
-  Variant step: forall (e: MachineEvent.t) (tid: Ident.t) (c1 c2: Configuration.t), Prop :=
-  | step_intro
-      e tid c1 lang st1 lc1 st3 lc3 gl3
-      (TID: IdentMap.find tid (Configuration.threads c1) = Some (existT _ lang st1, lc1))
-      (STEP: Thread.step (Global.max_reserved (Configuration.global c1)) true e
-                         (Thread.mk _ st1 lc1 (Configuration.global c1))
-                         (Thread.mk _ st3 lc3 gl3)):
-      step (ThreadEvent.get_machine_event_pf e) tid
-           c1
-           (Configuration.mk (IdentMap.add tid (existT _ _ st3, lc3) (Configuration.threads c1)) gl3)
+  Variant estep: forall (e: ThreadEvent.t) (tid: Ident.t) (c1 c2: Configuration.t), Prop :=
+    | estep_intro
+        e tid c1 lang st1 lc1 st3 lc3 gl3
+        (TID: IdentMap.find tid (Configuration.threads c1) = Some (existT _ lang st1, lc1))
+        (STEP: Thread.step (Global.max_reserved (Configuration.global c1)) true e
+                           (Thread.mk _ st1 lc1 (Configuration.global c1))
+                           (Thread.mk _ st3 lc3 gl3)):
+      estep e tid
+            c1
+            (Configuration.mk (IdentMap.add tid (existT _ _ st3, lc3) (Configuration.threads c1)) gl3)
   .
-  #[global] Hint Constructors step: core.
-
-  Variant normal_step (c1 c2: Configuration.t): Prop :=
-  | normal_step_intro
-      e tid
-      (STEP: step e tid c1 c2)
-      (EVENT: e <> MachineEvent.failure)
-  .
-  #[global] Hint Constructors normal_step: core.
+  #[global] Hint Constructors estep: core.
 
   Variant all_step (c1 c2: Configuration.t): Prop :=
-  | all_step_intro
-      e tid
-      (STEP: step e tid c1 c2)
+    | all_step_intro
+        e tid
+        (STEP: estep e tid c1 c2)
   .
   #[global] Hint Constructors all_step: core.
 
-  Variant opt_step: forall (e: MachineEvent.t) (tid: Ident.t) (c1 c2: Configuration.t), Prop :=
-  | step_none
-      tid c:
-      opt_step MachineEvent.silent tid c c
-  | step_some
-      e tid c1 c2
-      (STEP: step e tid c1 c2):
-      opt_step e tid c1 c2
-  .
-  #[global] Hint Constructors opt_step: core.
-
-  Definition tau_step := union (step MachineEvent.silent).
-
-  Variant steps_failure (c1: Configuration.t): Prop :=
-  | steps_failure_intro
-      tid c2 c3
-      (STEPS: rtc tau_step c1 c2)
-      (FAILURE: step MachineEvent.failure tid c2 c3)
-  .
-  #[global] Hint Constructors steps_failure: core.
-
-  Lemma step_future
+  Lemma estep_future
         e tid c1 c2
-        (STEP: step e tid c1 c2)
+        (STEP: estep e tid c1 c2)
         (WF1: Configuration.wf c1):
     <<WF2: Configuration.wf c2>> /\
     <<GL_FUTURE: Global.future (Configuration.global c1) (Configuration.global c2)>>.
@@ -100,28 +72,6 @@ Module PFConfiguration.
       auto.
   Qed.
 
-  Lemma opt_step_future
-        e tid c1 c2
-        (STEP: opt_step e tid c1 c2)
-        (WF1: Configuration.wf c1):
-    <<WF2: Configuration.wf c2>> /\
-    <<GL_FUTURE: Global.future (Configuration.global c1) (Configuration.global c2)>>.
-  Proof.
-    inv STEP.
-    - splits; auto; refl.
-    - eapply step_future; eauto.
-  Qed.
-
-  Lemma normal_step_future
-        c1 c2
-        (STEP: normal_step c1 c2)
-        (WF1: Configuration.wf c1):
-    <<WF2: Configuration.wf c2>> /\
-    <<GL_FUTURE: Global.future (Configuration.global c1) (Configuration.global c2)>>.
-  Proof.
-    inv STEP. eauto using step_future.
-  Qed.
-
   Lemma all_step_future
         c1 c2
         (STEP: all_step c1 c2)
@@ -129,37 +79,7 @@ Module PFConfiguration.
     <<WF2: Configuration.wf c2>> /\
     <<GL_FUTURE: Global.future (Configuration.global c1) (Configuration.global c2)>>.
   Proof.
-    inv STEP. eauto using step_future.
-  Qed.
-
-  Lemma rtc_step_future
-        c1 c2
-        (STEPS: rtc tau_step c1 c2)
-        (WF1: Configuration.wf c1):
-    <<WF2: Configuration.wf c2>> /\
-    <<GL_FUTURE: Global.future (Configuration.global c1) (Configuration.global c2)>>.
-  Proof.
-    induction STEPS; i.
-    - splits; auto; refl.
-    - inv H.
-      exploit step_future; eauto. i. des.
-      exploit IHSTEPS; eauto. i. des.
-      splits; eauto; etrans; eauto.
-  Qed.
-
-  Lemma rtc_normal_step_future
-        c1 c2
-        (STEPS: rtc normal_step c1 c2)
-        (WF1: Configuration.wf c1):
-    <<WF2: Configuration.wf c2>> /\
-    <<GL_FUTURE: Global.future (Configuration.global c1) (Configuration.global c2)>>.
-  Proof.
-    induction STEPS; i.
-    - splits; auto; refl.
-    - inv H.
-      exploit step_future; eauto. i. des.
-      exploit IHSTEPS; eauto. i. des.
-      splits; eauto; etrans; eauto.
+    inv STEP. eauto using estep_future.
   Qed.
 
   Lemma rtc_all_step_future
@@ -172,8 +92,111 @@ Module PFConfiguration.
     induction STEPS; i.
     - splits; auto; refl.
     - inv H.
-      exploit step_future; eauto. i. des.
+      exploit estep_future; eauto. i. des.
       exploit IHSTEPS; eauto. i. des.
       splits; eauto; etrans; eauto.
   Qed.
+
+  Section PFConfiguration.
+    Variable get_machine_event: ThreadEvent.t -> MachineEvent.t.
+
+    Variant step: forall (e: MachineEvent.t) (tid: Ident.t) (c1 c2: Configuration.t), Prop :=
+      | step_intro
+          e tid c1 c2
+          (STEP: estep e tid c1 c2):
+        step (get_machine_event e) tid c1 c2
+    .
+
+    Variant normal_step (c1 c2: Configuration.t): Prop :=
+      | normal_step_intro
+          e tid
+          (STEP: step e tid c1 c2)
+          (EVENT: e <> MachineEvent.failure)
+    .
+
+    Variant opt_step: forall (e: MachineEvent.t) (tid: Ident.t) (c1 c2: Configuration.t), Prop :=
+      | step_none
+          tid c:
+        opt_step MachineEvent.silent tid c c
+      | step_some
+          e tid c1 c2
+          (STEP: step e tid c1 c2):
+        opt_step e tid c1 c2
+    .
+
+    Definition tau_step := union (step MachineEvent.silent).
+
+    Variant steps_failure (c1: Configuration.t): Prop :=
+      | steps_failure_intro
+          tid c2 c3
+          (STEPS: rtc tau_step c1 c2)
+          (FAILURE: step MachineEvent.failure tid c2 c3)
+    .
+
+    Lemma step_future
+          e tid c1 c2
+          (STEP: step e tid c1 c2)
+          (WF1: Configuration.wf c1):
+      <<WF2: Configuration.wf c2>> /\
+      <<GL_FUTURE: Global.future (Configuration.global c1) (Configuration.global c2)>>.
+    Proof.
+      inv STEP. eauto using estep_future.
+    Qed.
+
+    Lemma opt_step_future
+          e tid c1 c2
+          (STEP: opt_step e tid c1 c2)
+          (WF1: Configuration.wf c1):
+      <<WF2: Configuration.wf c2>> /\
+      <<GL_FUTURE: Global.future (Configuration.global c1) (Configuration.global c2)>>.
+    Proof.
+      inv STEP.
+      - splits; auto; refl.
+      - eapply step_future; eauto.
+    Qed.
+
+    Lemma normal_step_future
+          c1 c2
+          (STEP: normal_step c1 c2)
+          (WF1: Configuration.wf c1):
+      <<WF2: Configuration.wf c2>> /\
+      <<GL_FUTURE: Global.future (Configuration.global c1) (Configuration.global c2)>>.
+    Proof.
+      inv STEP. eauto using step_future.
+    Qed.
+
+    Lemma rtc_step_future
+          c1 c2
+          (STEPS: rtc tau_step c1 c2)
+          (WF1: Configuration.wf c1):
+      <<WF2: Configuration.wf c2>> /\
+      <<GL_FUTURE: Global.future (Configuration.global c1) (Configuration.global c2)>>.
+    Proof.
+      induction STEPS; i.
+      - splits; auto; refl.
+      - inv H.
+        exploit step_future; eauto. i. des.
+        exploit IHSTEPS; eauto. i. des.
+        splits; eauto; etrans; eauto.
+    Qed.
+
+    Lemma rtc_normal_step_future
+          c1 c2
+          (STEPS: rtc normal_step c1 c2)
+          (WF1: Configuration.wf c1):
+      <<WF2: Configuration.wf c2>> /\
+      <<GL_FUTURE: Global.future (Configuration.global c1) (Configuration.global c2)>>.
+    Proof.
+      induction STEPS; i.
+      - splits; auto; refl.
+      - inv H.
+        exploit step_future; eauto. i. des.
+        exploit IHSTEPS; eauto. i. des.
+        splits; eauto; etrans; eauto.
+    Qed.
+  End PFConfiguration.
 End PFConfiguration.
+#[export] Hint Constructors step: core.
+#[export] Hint Constructors normal_step: core.
+#[export] Hint Constructors opt_step: core.
+#[export] Hint Constructors steps_failure: core.
