src/model/Thread.v
@@ -6,6 +6,7 @@ From Paco Require Import paco.
 
 From PromisingLib Require Import Axioms.
 From PromisingLib Require Import Basic.
+From PromisingLib Require Import Loc.
 From PromisingLib Require Import DataStructure.
 From PromisingLib Require Import DenseOrder.
 From PromisingLib Require Import Language.
@@ -25,29 +26,29 @@ Require Import Local.
 Set Implicit Arguments.
 
 
-Variant tau T (step: forall (e:ThreadEvent.t) (e1 e2:T), Prop) (e1 e2:T): Prop :=
+Variant tau T (step: forall (e:ThreadEvent.t) (th1 th2:T), Prop) (th1 th2:T): Prop :=
 | tau_intro
     e
-    (TSTEP: step e e1 e2)
+    (TSTEP: step e th1 th2)
     (EVENT: ThreadEvent.get_machine_event e = MachineEvent.silent)
 .
 #[export] Hint Constructors tau: core.
 
-Variant union E T (step: forall (e:E) (e1 e2:T), Prop) (e1 e2:T): Prop :=
+Variant union E T (step: forall (e:E) (th1 th2:T), Prop) (th1 th2:T): Prop :=
 | union_intro
     e
-    (USTEP: step e e1 e2)
+    (USTEP: step e th1 th2)
 .
 #[export] Hint Constructors union: core.
 
-Lemma tau_mon T (step1 step2: forall (e:ThreadEvent.t) (e1 e2:T), Prop)
+Lemma tau_mon T (step1 step2: forall (e:ThreadEvent.t) (th1 th2:T), Prop)
       (STEP: step1 <3= step2):
   tau step1 <2= tau step2.
 Proof.
   i. inv PR. econs; eauto.
 Qed.
 
-Lemma union_mon E T (step1 step2: forall (e:E) (e1 e2:T), Prop)
+Lemma union_mon E T (step1 step2: forall (e:E) (th1 th2:T), Prop)
       (STEP: step1 <3= step2):
   union step1 <2= union step2.
 Proof.
@@ -71,23 +72,23 @@ Module Thread.
       global: Global.t;
     }.
 
-    Variant step: forall (pf: bool) (e: ThreadEvent.t) (e1 e2: t), Prop :=
+    Variant step: forall (pf: bool) (e: ThreadEvent.t) (th1 th2: t), Prop :=
     | step_internal
         e st lc1 gl1 lc2 gl2
         (STEP: Local.internal_step e lc1 gl1 lc2 gl2):
       step false e (mk st lc1 gl1) (mk st lc2 gl2)
     | step_program
-        e st1 lc1 gl1 st2 lc2 gl2
-        (STATE: Language.step lang (ThreadEvent.get_program_event e) st1 st2)
+        e sth1 lc1 gl1 sth2 lc2 gl2
+        (STATE: Language.step lang (ThreadEvent.get_program_event e) sth1 sth2)
         (STEP: Local.program_step reserved e lc1 gl1 lc2 gl2):
-        step true e (mk st1 lc1 gl1) (mk st2 lc2 gl2)
+        step true e (mk sth1 lc1 gl1) (mk sth2 lc2 gl2)
     .
     #[local] Hint Constructors step: core.
 
-    Variant step_allpf (e:ThreadEvent.t) (e1 e2:t): Prop :=
+    Variant step_allpf (e:ThreadEvent.t) (th1 th2:t): Prop :=
     | step_nopf_intro
         pf
-        (STEP: step pf e e1 e2)
+        (STEP: step pf e th1 th2)
     .
     #[local] Hint Constructors step_allpf: core.
 
@@ -105,23 +106,23 @@ Module Thread.
     Definition all_step := union step_allpf.
     Hint Unfold all_step: core.
 
-    Variant opt_step: forall (e:ThreadEvent.t) (e1 e2:t), Prop :=
+    Variant opt_step: forall (e:ThreadEvent.t) (th1 th2:t), Prop :=
     | step_none
         e:
         opt_step ThreadEvent.silent e e
     | step_some
-        pf e e1 e2
-        (STEP: step pf e e1 e2):
-        opt_step e e1 e2
+        pf e th1 th2
+        (STEP: step pf e th1 th2):
+        opt_step e th1 th2
     .
     #[local] Hint Constructors opt_step: core.
 
     Lemma tau_opt_tau
-          e1 e2 e3 e
-          (STEPS: rtc tau_step e1 e2)
-          (STEP: opt_step e e2 e3)
+          th1 th2 th3 e
+          (STEPS: rtc tau_step th1 th2)
+          (STEP: opt_step e th2 th3)
           (EVENT: ThreadEvent.get_machine_event e = MachineEvent.silent):
-      rtc tau_step e1 e3.
+      rtc tau_step th1 th3.
     Proof.
       induction STEPS.
       - inv STEP; eauto.
@@ -129,10 +130,10 @@ Module Thread.
     Qed.
 
     Lemma tau_opt_all
-          e1 e2 e3 e
-          (STEPS: rtc tau_step e1 e2)
-          (STEP: opt_step e e2 e3):
-      rtc all_step e1 e3.
+          th1 th2 th3 e
+          (STEPS: rtc tau_step th1 th2)
+          (STEP: opt_step e th2 th3):
+      rtc all_step th1 th3.
     Proof.
       induction STEPS.
       - inv STEP; eauto.
@@ -142,11 +143,11 @@ Module Thread.
     Qed.
 
 
-    Variant steps_failure (e1: t): Prop :=
+    Variant steps_failure (th1: t): Prop :=
     | steps_failure_intro
-        e pf e2 e3
-        (STEPS: rtc tau_step e1 e2)
-        (STEP_FAILURE: step pf e e2 e3)
+        pf e th2 th3
+        (STEPS: rtc tau_step th1 th2)
+        (STEP_FAILURE: step pf e th2 th3)
         (EVENT_FAILURE: ThreadEvent.get_machine_event e = MachineEvent.failure)
     .
 
@@ -154,14 +155,14 @@ Module Thread.
     (* step_future *)
 
     Lemma step_future
-          pf e e1 e2
-          (STEP: step pf e e1 e2)
-          (LC_WF1: Local.wf (local e1) (global e1))
-          (GL_WF1: Global.wf (global e1)):
-      <<LC_WF2: Local.wf (local e2) (global e2)>> /\
-      <<GL_WF2: Global.wf (global e2)>> /\
-      <<TVIEW_FUTURE: TView.le (Local.tview (local e1)) (Local.tview (local e2))>> /\
-      <<GL_FUTURE: Global.future (global e1) (global e2)>>.
+          pf e th1 th2
+          (STEP: step pf e th1 th2)
+          (LC_WF1: Local.wf (local th1) (global th1))
+          (GL_WF1: Global.wf (global th1)):
+      <<LC_WF2: Local.wf (local th2) (global th2)>> /\
+      <<GL_WF2: Global.wf (global th2)>> /\
+      <<TVIEW_FUTURE: TView.le (Local.tview (local th1)) (Local.tview (local th2))>> /\
+      <<GL_FUTURE: Global.future (global th1) (global th2)>>.
     Proof.
       inv STEP; ss.
       - eapply Local.internal_step_future; eauto.
@@ -169,14 +170,14 @@ Module Thread.
     Qed.
 
     Lemma opt_step_future
-          e e1 e2
-          (STEP: opt_step e e1 e2)
-          (LC_WF1: Local.wf (local e1) (global e1))
-          (GL_WF1: Global.wf (global e1)):
-      <<LC_WF2: Local.wf (local e2) (global e2)>> /\
-      <<GL_WF2: Global.wf (global e2)>> /\
-      <<TVIEW_FUTURE: TView.le (Local.tview (local e1)) (Local.tview (local e2))>> /\
-      <<GL_FUTURE: Global.future (global e1) (global e2)>>.
+          e th1 th2
+          (STEP: opt_step e th1 th2)
+          (LC_WF1: Local.wf (local th1) (global th1))
+          (GL_WF1: Global.wf (global th1)):
+      <<LC_WF2: Local.wf (local th2) (global th2)>> /\
+      <<GL_WF2: Global.wf (global th2)>> /\
+      <<TVIEW_FUTURE: TView.le (Local.tview (local th1)) (Local.tview (local th2))>> /\
+      <<GL_FUTURE: Global.future (global th1) (global th2)>>.
     Proof.
       inv STEP.
       - esplits; eauto; refl.
@@ -184,14 +185,14 @@ Module Thread.
     Qed.
 
     Lemma rtc_all_step_future
-          e1 e2
-          (STEP: rtc all_step e1 e2)
-          (LC_WF1: Local.wf (local e1) (global e1))
-          (GL_WF1: Global.wf (global e1)):
-      <<LC_WF2: Local.wf (local e2) (global e2)>> /\
-      <<GL_WF2: Global.wf (global e2)>> /\
-      <<TVIEW_FUTURE: TView.le (Local.tview (local e1)) (Local.tview (local e2))>> /\
-      <<GL_FUTURE: Global.future (global e1) (global e2)>>.
+          th1 th2
+          (STEP: rtc all_step th1 th2)
+          (LC_WF1: Local.wf (local th1) (global th1))
+          (GL_WF1: Global.wf (global th1)):
+      <<LC_WF2: Local.wf (local th2) (global th2)>> /\
+      <<GL_WF2: Global.wf (global th2)>> /\
+      <<TVIEW_FUTURE: TView.le (Local.tview (local th1)) (Local.tview (local th2))>> /\
+      <<GL_FUTURE: Global.future (global th1) (global th2)>>.
     Proof.
       revert LC_WF1. induction STEP.
       - i. splits; ss; refl.
@@ -202,14 +203,14 @@ Module Thread.
     Qed.
 
     Lemma rtc_tau_step_future
-          e1 e2
-          (STEP: rtc tau_step e1 e2)
-          (LC_WF1: Local.wf (local e1) (global e1))
-          (GL_WF1: Global.wf (global e1)):
-      <<LC_WF2: Local.wf (local e2) (global e2)>> /\
-      <<GL_WF2: Global.wf (global e2)>> /\
-      <<TVIEW_FUTURE: TView.le (Local.tview (local e1)) (Local.tview (local e2))>> /\
-      <<GL_FUTURE: Global.future (global e1) (global e2)>>.
+          th1 th2
+          (STEP: rtc tau_step th1 th2)
+          (LC_WF1: Local.wf (local th1) (global th1))
+          (GL_WF1: Global.wf (global th1)):
+      <<LC_WF2: Local.wf (local th2) (global th2)>> /\
+      <<GL_WF2: Global.wf (global th2)>> /\
+      <<TVIEW_FUTURE: TView.le (Local.tview (local th1)) (Local.tview (local th2))>> /\
+      <<GL_FUTURE: Global.future (global th1) (global th2)>>.
     Proof.
       apply rtc_all_step_future; auto.
       eapply rtc_implies; [|eauto].
@@ -217,30 +218,30 @@ Module Thread.
     Qed.
 
     Lemma step_nonpf_future
-          e e1 e2
-          (STEP: step false e e1 e2)
-          (LC_WF1: Local.wf (local e1) (global e1))
-          (GL_WF1: Global.wf (global e1)):
-      <<LC_WF2: Local.wf (local e2) (global e2)>> /\
-      <<GL_WF2: Global.wf (global e2)>> /\
-      <<TVIEW_FUTURE: TView.le (Local.tview (local e1)) (Local.tview (local e2))>> /\
-      <<GL_FUTURE: Global.future (global e1) (global e2)>> /\
-      <<STATE: (state e1) = (state e2)>>.
+          e th1 th2
+          (STEP: step false e th1 th2)
+          (LC_WF1: Local.wf (local th1) (global th1))
+          (GL_WF1: Global.wf (global th1)):
+      <<LC_WF2: Local.wf (local th2) (global th2)>> /\
+      <<GL_WF2: Global.wf (global th2)>> /\
+      <<TVIEW_FUTURE: TView.le (Local.tview (local th1)) (Local.tview (local th2))>> /\
+      <<GL_FUTURE: Global.future (global th1) (global th2)>> /\
+      <<STATE: (state th1) = (state th2)>>.
     Proof.
       exploit step_future; eauto. i. des.
       inv STEP. inv STEP0; esplits; ss.
     Qed.
 
     Lemma rtc_step_nonpf_future
-          e1 e2
-          (STEP: rtc (union (step false)) e1 e2)
-          (LC_WF1: Local.wf (local e1) (global e1))
-          (GL_WF1: Global.wf (global e1)):
-      <<LC_WF2: Local.wf (local e2) (global e2)>> /\
-      <<GL_WF2: Global.wf (global e2)>> /\
-      <<TVIEW_FUTURE: TView.le (Local.tview (local e1)) (Local.tview (local e2))>> /\
-      <<GL_FUTURE: Global.future (global e1) (global e2)>> /\
-      <<STATE: (state e1) = (state e2)>>.
+          th1 th2
+          (STEP: rtc (union (step false)) th1 th2)
+          (LC_WF1: Local.wf (local th1) (global th1))
+          (GL_WF1: Global.wf (global th1)):
+      <<LC_WF2: Local.wf (local th2) (global th2)>> /\
+      <<GL_WF2: Global.wf (global th2)>> /\
+      <<TVIEW_FUTURE: TView.le (Local.tview (local th1)) (Local.tview (local th2))>> /\
+      <<GL_FUTURE: Global.future (global th1) (global th2)>> /\
+      <<STATE: (state th1) = (state th2)>>.
     Proof.
       revert LC_WF1. induction STEP.
       - i. splits; ss; refl.
@@ -253,10 +254,10 @@ Module Thread.
     (* step_inhabited *)
 
     Lemma step_inhabited
-          pf e e1 e2
-          (STEP: step pf e e1 e2)
-          (INHABITED1: Memory.inhabited (Global.memory (global e1))):
-      <<INHABITED2: Memory.inhabited (Global.memory (global e2))>>.
+          pf e th1 th2
+          (STEP: step pf e th1 th2)
+          (INHABITED1: Memory.inhabited (Global.memory (global th1))):
+      <<INHABITED2: Memory.inhabited (Global.memory (global th2))>>.
     Proof.
       inv STEP.
       - eapply Local.internal_step_inhabited; eauto.
@@ -267,12 +268,12 @@ Module Thread.
     (* step_disjoint *)
 
     Lemma step_disjoint
-          pf e e1 e2 lc
-          (STEP: step pf e e1 e2)
-          (DISJOINT1: Local.disjoint (local e1) lc)
-          (LC_WF: Local.wf lc (global e1)):
-      <<DISJOINT2: Local.disjoint (local e2) lc>> /\
-      <<LC_WF: Local.wf lc (global e2)>>.
+          pf e th1 th2 lc
+          (STEP: step pf e th1 th2)
+          (DISJOINTH1: Local.disjoint (local th1) lc)
+          (LC_WF: Local.wf lc (global th1)):
+      <<DISJOINTH2: Local.disjoint (local th2) lc>> /\
+      <<LC_WF: Local.wf lc (global th2)>>.
     Proof.
       inv STEP.
       - eapply Local.internal_step_disjoint; eauto.
@@ -280,12 +281,12 @@ Module Thread.
     Qed.
 
     Lemma opt_step_disjoint
-          e e1 e2 lc
-          (STEP: opt_step e e1 e2)
-          (DISJOINT1: Local.disjoint (local e1) lc)
-          (LC_WF: Local.wf lc (global e1)):
-      <<DISJOINT2: Local.disjoint (local e2) lc>> /\
-      <<LC_WF: Local.wf lc (global e2)>>.
+          e th1 th2 lc
+          (STEP: opt_step e th1 th2)
+          (DISJOINTH1: Local.disjoint (local th1) lc)
+          (LC_WF: Local.wf lc (global th1)):
+      <<DISJOINTH2: Local.disjoint (local th2) lc>> /\
+      <<LC_WF: Local.wf lc (global th2)>>.
     Proof.
       inv STEP.
       - esplits; eauto.
@@ -293,26 +294,26 @@ Module Thread.
     Qed.
 
     Lemma rtc_all_step_disjoint
-          e1 e2 lc
-          (STEP: rtc all_step e1 e2)
-          (DISJOINT1: Local.disjoint (local e1) lc)
-          (LC_WF: Local.wf lc (global e1)):
-      <<DISJOINT2: Local.disjoint (local e2) lc>> /\
-      <<LC_WF: Local.wf lc (global e2)>>.
+          th1 th2 lc
+          (STEP: rtc all_step th1 th2)
+          (DISJOINTH1: Local.disjoint (local th1) lc)
+          (LC_WF: Local.wf lc (global th1)):
+      <<DISJOINTH2: Local.disjoint (local th2) lc>> /\
+      <<LC_WF: Local.wf lc (global th2)>>.
     Proof.
-      revert DISJOINT1 LC_WF. induction STEP; eauto. i.
+      revert DISJOINTH1 LC_WF. induction STEP; eauto. i.
       inv H. inv USTEP.
       exploit step_disjoint; eauto. i. des.
       exploit IHSTEP; eauto.
     Qed.
 
     Lemma rtc_tau_step_disjoint
-          e1 e2 lc
-          (STEP: rtc tau_step e1 e2)
-          (DISJOINT1: Local.disjoint (local e1) lc)
-          (LC_WF: Local.wf lc (global e1)):
-      <<DISJOINT2: Local.disjoint (local e2) lc>> /\
-      <<LC_WF: Local.wf lc (global e2)>>.
+          th1 th2 lc
+          (STEP: rtc tau_step th1 th2)
+          (DISJOINTH1: Local.disjoint (local th1) lc)
+          (LC_WF: Local.wf lc (global th1)):
+      <<DISJOINTH2: Local.disjoint (local th2) lc>> /\
+      <<LC_WF: Local.wf lc (global th2)>>.
     Proof.
       eapply rtc_all_step_disjoint; cycle 1; eauto.
       eapply rtc_implies; [|eauto].
@@ -320,10 +321,10 @@ Module Thread.
     Qed.
 
     (* Lemma program_step_promises_bot *)
-    (*       e e1 e2 *)
-    (*       (STEP: program_step e e1 e2) *)
-    (*       (PROMISES: (Local.promises (local e1)) = Memory.bot): *)
-    (*   (Local.promises (local e2)) = Memory.bot. *)
+    (*       e th1 th2 *)
+    (*       (STEP: program_step e th1 th2) *)
+    (*       (PROMISES: (Local.promises (local th1)) = Memory.bot): *)
+    (*   (Local.promises (local th2)) = Memory.bot. *)
     (* Proof. *)
     (*   inv STEP. eapply Local.program_step_promises_bot; eauto. *)
     (* Qed. *)
@@ -331,41 +332,41 @@ Module Thread.
 
     (* reserve & cancel steps *)
 
-    (* Variant reserve_step (e1 e2:t): Prop := *)
+    (* Variant reserve_step (th1 th2:t): Prop := *)
     (* | reserve_step_intro *)
     (*     pf loc from to *)
-    (*     (STEP: step pf (ThreadEvent.promise loc from to Message.reserve Memory.op_kind_add) e1 e2) *)
+    (*     (STEP: step pf (ThreadEvent.promise loc from to Message.reserve Memory.op_kind_add) th1 th2) *)
     (* . *)
     (* Hint Constructors reserve_step: core. *)
 
-    (* Variant cancel_step (e1 e2:t): Prop := *)
+    (* Variant cancel_step (th1 th2:t): Prop := *)
     (* | cancel_step_intro *)
     (*     pf loc from to *)
-    (*     (STEP: step pf (ThreadEvent.promise loc from to Message.reserve Memory.op_kind_cancel) e1 e2) *)
+    (*     (STEP: step pf (ThreadEvent.promise loc from to Message.reserve Memory.op_kind_cancel) th1 th2) *)
     (* . *)
     (* Hint Constructors cancel_step: core. *)
 
-    (* Lemma reserve_step_tau_step e1 e2 *)
-    (*       (RESERVE: reserve_step e1 e2) *)
+    (* Lemma reserve_step_tau_step th1 th2 *)
+    (*       (RESERVE: reserve_step th1 th2) *)
     (*   : *)
-    (*     tau_step e1 e2. *)
+    (*     tau_step th1 th2. *)
     (* Proof. *)
     (*   inv RESERVE. econs; eauto. *)
     (* Qed. *)
 
-    (* Lemma cancel_step_tau_step e1 e2 *)
-    (*       (CANCEL: cancel_step e1 e2) *)
+    (* Lemma cancel_step_tau_step th1 th2 *)
+    (*       (CANCEL: cancel_step th1 th2) *)
     (*   : *)
-    (*     tau_step e1 e2. *)
+    (*     tau_step th1 th2. *)
     (* Proof. *)
     (*   inv CANCEL. econs; eauto. *)
     (* Qed. *)
 
     (* Lemma reservation_event_reserve_or_cancel_step *)
-    (*       (e1 e2: t) pf e *)
+    (*       (th1 th2: t) pf e *)
     (*       (RESERVATION: ThreadEvent.is_reservation_event e) *)
-    (*       (STEP: step pf e e1 e2): *)
-    (*     reserve_step e1 e2 \/ cancel_step e1 e2. *)
+    (*       (STEP: step pf e th1 th2): *)
+    (*     reserve_step th1 th2 \/ cancel_step th1 th2. *)
     (* Proof. *)
     (*   dup STEP. inv STEP. *)
     (*   - inv STEP1. inv LOCAL. ss. des_ifs. inv PROMISE; ss; eauto. *)
@@ -373,17 +374,17 @@ Module Thread.
     (* Qed. *)
 
     (* Lemma rtc_reserve_step_future *)
-    (*       e1 e2 *)
-    (*       (STEP: rtc reserve_step e1 e2) *)
-    (*       (WF1: Local.wf (local e1) (memory e1)) *)
-    (*       (SC1: Memory.closed_timemap (sc e1) (memory e1)) *)
-    (*       (CLOSED1: Memory.closed (memory e1)): *)
-    (*   <<WF2: Local.wf (local e2) (memory e2)>> /\ *)
-    (*   <<SC2: Memory.closed_timemap (sc e2) (memory e2)>> /\ *)
-    (*   <<CLOSED2: Memory.closed (memory e2)>> /\ *)
-    (*   <<TVIEW_FUTURE: TView.le (Local.tview (local e1)) (Local.tview (local e2))>> /\ *)
-    (*   <<SC_FUTURE: TimeMap.le (sc e1) (sc e2)>> /\ *)
-    (*   <<MEM_FUTURE: Memory.future (memory e1) (memory e2)>>. *)
+    (*       th1 th2 *)
+    (*       (STEP: rtc reserve_step th1 th2) *)
+    (*       (WF1: Local.wf (local th1) (memory th1)) *)
+    (*       (SC1: Memory.closed_timemap (sc th1) (memory th1)) *)
+    (*       (CLOSED1: Memory.closed (memory th1)): *)
+    (*   <<WF2: Local.wf (local th2) (memory th2)>> /\ *)
+    (*   <<SC2: Memory.closed_timemap (sc th2) (memory th2)>> /\ *)
+    (*   <<CLOSED2: Memory.closed (memory th2)>> /\ *)
+    (*   <<TVIEW_FUTURE: TView.le (Local.tview (local th1)) (Local.tview (local th2))>> /\ *)
+    (*   <<SC_FUTURE: TimeMap.le (sc th1) (sc th2)>> /\ *)
+    (*   <<MEM_FUTURE: Memory.future (memory th1) (memory th2)>>. *)
     (* Proof. *)
     (*   apply rtc_all_step_future; auto. *)
     (*   eapply rtc_implies; [|eauto]. *)
@@ -391,17 +392,17 @@ Module Thread.
     (* Qed. *)
 
     (* Lemma rtc_cancel_step_future *)
-    (*       e1 e2 *)
-    (*       (STEP: rtc cancel_step e1 e2) *)
-    (*       (WF1: Local.wf (local e1) (memory e1)) *)
-    (*       (SC1: Memory.closed_timemap (sc e1) (memory e1)) *)
-    (*       (CLOSED1: Memory.closed (memory e1)): *)
-    (*   <<WF2: Local.wf (local e2) (memory e2)>> /\ *)
-    (*   <<SC2: Memory.closed_timemap (sc e2) (memory e2)>> /\ *)
-    (*   <<CLOSED2: Memory.closed (memory e2)>> /\ *)
-    (*   <<TVIEW_FUTURE: TView.le (Local.tview (local e1)) (Local.tview (local e2))>> /\ *)
-    (*   <<SC_FUTURE: TimeMap.le (sc e1) (sc e2)>> /\ *)
-    (*   <<MEM_FUTURE: Memory.future (memory e1) (memory e2)>>. *)
+    (*       th1 th2 *)
+    (*       (STEP: rtc cancel_step th1 th2) *)
+    (*       (WF1: Local.wf (local th1) (memory th1)) *)
+    (*       (SC1: Memory.closed_timemap (sc th1) (memory th1)) *)
+    (*       (CLOSED1: Memory.closed (memory th1)): *)
+    (*   <<WF2: Local.wf (local th2) (memory th2)>> /\ *)
+    (*   <<SC2: Memory.closed_timemap (sc th2) (memory th2)>> /\ *)
+    (*   <<CLOSED2: Memory.closed (memory th2)>> /\ *)
+    (*   <<TVIEW_FUTURE: TView.le (Local.tview (local th1)) (Local.tview (local th2))>> /\ *)
+    (*   <<SC_FUTURE: TimeMap.le (sc th1) (sc th2)>> /\ *)
+    (*   <<MEM_FUTURE: Memory.future (memory th1) (memory th2)>>. *)
     (* Proof. *)
     (*   apply rtc_all_step_future; auto. *)
     (*   eapply rtc_implies; [|eauto]. *)
@@ -412,13 +413,13 @@ Module Thread.
 
   (* consistency *)
 
-  Variant consistent {lang: language} (e: t lang): Prop :=
+  Variant consistent {lang: language} (th: t lang): Prop :=
   | consistent_failure
-      (FAILURE: @steps_failure lang (Global.max_reserved (global e)) e)
+      (FAILURE: @steps_failure lang (Global.max_reserved (global th)) th)
   | consistent_promises
-      e2
-      (STEPS: rtc (@tau_step lang (Global.max_reserved (global e))) e e2)
-      (PROMISES: (Local.promises (local e2)) = BoolMap.bot)
+      th2
+      (STEPS: rtc (@tau_step lang (Global.max_reserved (global th))) th th2)
+      (PROMISES: (Local.promises (local th2)) = BoolMap.bot)
   .
 End Thread.
 #[export] Hint Constructors Thread.step: core.
