src/model/Cell.v
@@ -4,9 +4,9 @@ From sflib Require Import sflib.
 
 From PromisingLib Require Import Axioms.
 From PromisingLib Require Import Basic.
+From PromisingLib Require Import Loc.
 From PromisingLib Require Import DataStructure.
 From PromisingLib Require Import DenseOrder.
-From PromisingLib Require Import Loc.
 From PromisingLib Require Import Event.
 
 Require Import Time.
