src/model/Configuration.v
@@ -3,6 +3,7 @@ From Paco Require Import paco.
 
 From PromisingLib Require Import Axioms.
 From PromisingLib Require Import Basic.
+From PromisingLib Require Import Loc.
 From PromisingLib Require Import DataStructure.
 From PromisingLib Require Import DenseOrder.
 From PromisingLib Require Import Language.
