src/model/Memory.v
@@ -1,12 +1,12 @@
-Require Import RelationClasses.
+\Require Import RelationClasses.
 
 From sflib Require Import sflib.
 
 From PromisingLib Require Import Axioms.
 From PromisingLib Require Import Basic.
+From PromisingLib Require Import Loc.
 From PromisingLib Require Import DataStructure.
 From PromisingLib Require Import DenseOrder.
-From PromisingLib Require Import Loc.
 From PromisingLib Require Import Event.
 
 Require Import Time.
